relabel implementation with bodyless lemma's

Flow.dfy
@@ -4,19 +4,22 @@ module FlowGraph {
   import Graph
 
   predicate ValidFlowMatrixShape(V: nat, flow: array2<nat>)
-    reads flow
   {
     flow.Length0 == V && flow.Length1 == V
   }
 
+  predicate ValidCapacityMatrixShape(V: nat, capacity: array2<nat>)
+  {
+    capacity.Length0 == V &&
+    capacity.Length1 == V
+  }
+
   predicate ValidExcessShape(V: nat, excess: array<int>)
-    reads excess
   {
     excess.Length == V
   }
 
   predicate ValidHeightShape(V: nat, height: array<nat>)
-    reads height
   {
     height.Length == V
   }
@@ -29,12 +32,17 @@ module FlowGraph {
     excess[u] > 0
   }
 
+  predicate NodeIsSourceOrSink(u: nat, s: nat, t: nat)
+  {
+    u == s || u == t
+  }
 
   function ResidualCapacity(V: nat, s: nat, t: nat, capacity: array2<nat>, flow: array2<nat>, u: nat, v: nat): nat
     reads capacity, flow
-    requires Graph.ValidGraph(V, s, t, capacity)
+    requires Graph.ValidGraph(V, s, t)
     requires ValidFlowMatrixShape(V, flow)
-    requires Graph.ValidEdge(V, u, v)
+    requires ValidCapacityMatrixShape(V, capacity)
+    requires Graph.ValidNode(V, u) && Graph.ValidNode(V, v)
     requires ValidFlow(V, s, t, capacity, flow)
   {
     capacity[u, v] - flow[u, v] + flow[v, u]
@@ -42,9 +50,10 @@ module FlowGraph {
 
   predicate EdgeInResidual(V: nat, s: nat, t: nat, capacity: array2<nat>, flow: array2<nat>, u: nat, v: nat)
     reads capacity, flow
-    requires Graph.ValidGraph(V, s, t, capacity)
+    requires Graph.ValidGraph(V, s, t)
     requires ValidFlowMatrixShape(V, flow)
-    requires Graph.ValidEdge(V, u, v)
+    requires ValidCapacityMatrixShape(V, capacity)
+    requires Graph.ValidNode(V, u) && Graph.ValidNode(V, v)
     requires ValidFlow(V, s, t, capacity, flow)
   {
     ResidualCapacity(V, s, t, capacity, flow, u, v) > 0
@@ -52,31 +61,82 @@ module FlowGraph {
 
   predicate ValidFlow(V: nat, s: nat, t: nat, capacity: array2<nat>, flow: array2<nat>)
     reads capacity, flow
-    requires Graph.ValidGraph(V, s, t, capacity)
+    requires Graph.ValidGraph(V, s, t)
     requires ValidFlowMatrixShape(V, flow)
+    requires ValidCapacityMatrixShape(V, capacity)
   {
-    forall u, v :: 0 <= u < V && 0 <= v < V ==>
-                     0 <= flow[u, v] <= capacity[u, v]
+    forall u, v :: (0 <= u < V && 0 <= v < V) ==>
+                     (0 <= flow[u, v] <= capacity[u, v])
   }
 
-  predicate ValidPreflow(V: nat, s: nat, t: nat, capacity: array2<nat>, excess: array<int>)
-    reads capacity, excess
-    requires Graph.ValidGraph(V, s, t, capacity)
+  predicate ValidPreflow(V: nat, s: nat, t: nat, excess: array<int>)
+    reads excess
+    requires Graph.ValidGraph(V, s, t)
     requires ValidExcessShape(V, excess)
   {
-    forall u :: 0 <= u < V && u != s && u != t ==> excess[u] >= 0
+    forall u :: (0 <= u < V && !NodeIsSourceOrSink(u, s, t)) ==> excess[u] >= 0
   }
 
   predicate ValidLabeling(V: nat, s: nat, t: nat, capacity: array2<nat>, flow: array2<nat>, height: array<nat>)
     reads capacity, flow, height
-    requires Graph.ValidGraph(V, s, t, capacity)
+    requires Graph.ValidGraph(V, s, t)
     requires ValidFlowMatrixShape(V, flow)
+    requires ValidCapacityMatrixShape(V, capacity)
     requires ValidHeightShape(V, height)
     requires ValidFlow(V, s, t, capacity, flow)
   {
     height[s] == V &&
     height[t] == 0 &&
-    (forall u, v :: 0 <= u < V && 0 <= v < V && EdgeInResidual(V, s, t, capacity, flow, u, v) ==>
-                      height[u] <= height[v] + 1)
+    (forall u, v :: (0 <= u < V && 0 <= v < V && EdgeInResidual(V, s, t, capacity, flow, u, v)) ==>
+                      (height[u] <= height[v] + 1))
   }
+
+  predicate IsResidualPath(V: nat, s: nat, t: nat, capacity: array2<nat>, flow: array2<nat>, p: seq<nat>)
+    reads capacity, flow
+    requires Graph.ValidGraph(V, s, t)
+    requires ValidFlowMatrixShape(V, flow)
+    requires ValidCapacityMatrixShape(V, capacity)
+    requires ValidFlow(V, s, t, capacity, flow)
+  {
+    |p| > 0 &&
+    (forall i :: (0 <= i < |p|) ==>
+                   (Graph.ValidNode(V, p[i]))) &&
+    (forall i :: (0 <= i < |p| - 1) ==>
+                   (EdgeInResidual(V, s, t, capacity, flow, p[i], p[i+1])))
+  }
+
+  predicate IsSimpleResidualPath(V: nat, s: nat, t: nat, capacity: array2<nat>, flow: array2<nat>, p: seq<nat>)
+    reads capacity, flow
+    requires Graph.ValidGraph(V, s, t)
+    requires ValidFlowMatrixShape(V, flow)
+    requires ValidCapacityMatrixShape(V, capacity)
+    requires ValidFlow(V, s, t, capacity, flow)
+  {
+    IsResidualPath(V, s, t, capacity, flow, p) && Graph.NodeSequenceHasNoDuplicates(p)
+  }
+
+  lemma Lemma_ActiveNodeHasPathToSource(V: nat, s: nat, t: nat, capacity: array2<nat>, flow: array2<nat>, excess: array<int>, u: nat)
+    requires Graph.ValidGraph(V, s, t)
+    requires ValidFlowMatrixShape(V, flow)
+    requires ValidCapacityMatrixShape(V, capacity)
+    requires ValidExcessShape(V, excess)
+    requires ValidPreflow(V, s, t, excess)
+    requires Graph.ValidNode(V, u) && !NodeIsSourceOrSink(u, s, t)
+    requires NodeIsActive(V, u, excess)
+    requires ValidFlow(V, s, t, capacity, flow)
+    ensures exists p :: IsSimpleResidualPath(V, s, t, capacity, flow, p) && p[0] == u && p[|p|-1] == s
+
+  lemma Lemma_PathTelescopingHeight(V: nat, s: nat, t: nat, capacity: array2<nat>, flow: array2<nat>, height: array<nat>, p: seq<nat>)
+    requires |p| >= 1
+    requires Graph.ValidNode(V, p[0]) && Graph.ValidNode(V, p[|p| - 1])
+    requires Graph.ValidGraph(V, s, t)
+    requires ValidFlowMatrixShape(V, flow)
+    requires ValidCapacityMatrixShape(V, capacity)
+    requires ValidHeightShape(V, height)
+    requires ValidFlow(V, s, t, capacity, flow)
+    requires ValidLabeling(V, s, t, capacity, flow, height)
+
+    requires IsResidualPath(V, s, t, capacity, flow, p)
+
+    ensures height[p[0]] <= height[p[|p| - 1]] + |p| - 1
 }
