PushRelabel.dfy
@@ -15,17 +15,11 @@ module Algorithm {
     var height: array<nat>
     var excess: array<int>
 
-    var buckets: array<seq<nat>>
+    var buckets: array<set<nat>>
     var max_height: int
 
-    predicate NodeIsSourceOrSink(u: nat)
-      reads this
-    {
-      u == s || u == t
-    }
-
     predicate ValidBucketsStructure()
-      reads this, buckets
+      reads this
     {
       buckets.Length == 2 * V
     }
@@ -37,17 +31,19 @@ module Algorithm {
       requires ValidBucketsStructure()
     {
       -1 <= max_height < 2 * V &&
-      (forall u :: 0 <= u < V && u != s && u != t && excess[u] > 0 ==>
+      (forall u :: (0 <= u < V && u != s && u != t && excess[u] > 0) ==>
                      height[u] <= max_height) &&
-      (forall u :: 0 <= u < V && u != s && u != t && excess[u] > 0 ==>
-                     u in buckets[height[u]])
+      (forall u :: (0 <= u < V && u != s && u != t && excess[u] > 0) ==>
+                     u in buckets[height[u]]) &&
+      (forall h, u :: (0 <= h < 2 * V && 0 <= u < V && u in buckets[h]) ==> height[u] == h)
     }
 
     predicate ValidStructure()
-      reads this, capacity, flow, height, excess, buckets
+      reads this
     {
-      Graph.ValidGraph(V, s, t, capacity) &&
+      Graph.ValidGraph(V, s, t) &&
       FlowGraph.ValidFlowMatrixShape(V, flow) &&
+      FlowGraph.ValidCapacityMatrixShape(V, capacity) &&
       FlowGraph.ValidHeightShape(V, height) &&
       FlowGraph.ValidExcessShape(V, excess) &&
       ValidBucketsStructure()
@@ -58,15 +54,16 @@ module Algorithm {
     {
       ValidStructure() &&
       FlowGraph.ValidFlow(V, s, t, capacity, flow) &&
-      FlowGraph.ValidPreflow(V, s, t, capacity, excess) &&
+      FlowGraph.ValidPreflow(V, s, t, excess) &&
       FlowGraph.ValidLabeling(V, s, t, capacity, flow, height) &&
       ValidBuckets()
     }
 
     function ResidualCapacity(u: nat, v: nat): nat
       reads this, capacity, flow
-      requires Graph.ValidGraph(V, s, t, capacity)
+      requires Graph.ValidGraph(V, s, t)
       requires FlowGraph.ValidFlowMatrixShape(V, flow)
+      requires FlowGraph.ValidCapacityMatrixShape(V, capacity)
       requires FlowGraph.ValidFlow(V, s, t, capacity, flow)
       requires Graph.ValidNode(V, u) && Graph.ValidNode(V, v)
     {
@@ -78,7 +75,7 @@ module Algorithm {
 
       // Preconditions for a valid push:
       requires Graph.ValidNode(V, u) && Graph.ValidNode(V, v)   // u and v must be nodes in the Graph
-      requires !NodeIsSourceOrSink(u)                           // u cannot be equal to the source or sink
+      requires !FlowGraph.NodeIsSourceOrSink(u, s, t)           // u cannot be equal to the source or sink
       requires FlowGraph.NodeIsActive(V, u, excess)             // u must be active
       requires ResidualCapacity(u, v) > 0                       // There must be pipe space
       requires height[u] == height[v] + 1                       // Water must flow exactly one step downhill
@@ -114,12 +111,12 @@ module Algorithm {
       excess[v] := excess[v] + push_val;
 
       // Update the Highest-Label Buckets
-      // If v was NOT active, and is not s or t (which implies it is active), it enters the buckets.
-      if (!old_v_active && !NodeIsSourceOrSink(v)) {
+      // If v was NOT active, and is not s or t (which implies it is active now), it enters the buckets.
+      if (!old_v_active && !FlowGraph.NodeIsSourceOrSink(v, s, t)) {
         assert FlowGraph.NodeIsActive(V, v, excess);
 
-        buckets[height[v]] := buckets[height[v]] + [v];
-        // We don't need to update max_height here because water flows downhill!
+        buckets[height[v]] := buckets[height[v]] + {v};
+        // We don't need to update max_height here because water flows downhill
         // height[v] is strictly less than height[u], so it cannot become the new max_height.
       }
     }
@@ -129,7 +126,7 @@ module Algorithm {
 
       // Preconditions for a valid relabel:
       requires Graph.ValidNode(V, u)                  // u must be a node in the Graph
-      requires !NodeIsSourceOrSink(u)                 // u cannot be equal to the source or sink
+      requires !FlowGraph.NodeIsSourceOrSink(u, s, t) // u cannot be equal to the source or sink
       requires FlowGraph.NodeIsActive(V, u, excess)   // u must be active
       // u cannot be relabeled if it has a downhill neighbor
       requires forall v :: 0 <= v < V && ResidualCapacity(u, v) > 0 ==> height[u] <= height[v]
@@ -140,38 +137,72 @@ module Algorithm {
       modifies this, height, buckets
     {
       // Find the lowest neighbor in the residual graph
-      // We initialize min_h to an impossibly high value (2 * V)
-      var min_h: nat := 2 * V;
+      // We initialize minHeightNeighbourOfU to an impossibly high value (2 * V)
+      var minHeightNeighbourOfU: nat := 2 * V;
       var v := 0;
 
       while (v < V)
         invariant 0 <= v <= V
-        invariant min_h <= 2 * V
-        // Loop invariant needed here to prove we find the actual minimum
-        invariant forall k :: 0 <= k < v && ResidualCapacity(u, k) > 0 ==> min_h <= height[k]
+        invariant minHeightNeighbourOfU <= 2 * V
+        invariant forall k :: 0 <= k < v && ResidualCapacity(u, k) > 0 ==> minHeightNeighbourOfU <= height[k]
 
-        // Because u had no downhill neighbors, height[u] MUST be <= min_h.
+        // Because u had no downhill neighbors, height[u] MUST be <= minHeightNeighbourOfU.
         // invariant so that Dafny does not forget
-        invariant height[u] <= min_h
+        invariant height[u] <= minHeightNeighbourOfU
       {
         if (ResidualCapacity(u, v) > 0) {
-          if (height[v] < min_h) {
-            min_h := height[v];
+          if (height[v] < minHeightNeighbourOfU) {
+            minHeightNeighbourOfU := height[v];
           }
         }
         v := v + 1;
       }
-      // Assert min_h is actual minimum
-      assert forall k :: 0 <= k < V && ResidualCapacity(u, k) > 0 ==> min_h <= height[k];
+      // Assert minHeightNeighbourOfU is actual minimum
+      assert forall k :: 0 <= k < V && ResidualCapacity(u, k) > 0 ==> minHeightNeighbourOfU <= height[k];
 
-      // (TODO: Lemma to prove this is correct)
-      assume min_h < 2 * V - 1;
+      // Prove a path to the source exists from u
+      FlowGraph.Lemma_ActiveNodeHasPathToSource(V, s, t, capacity, flow, excess, u);
+      // Extract that path
+      ghost var pathToSource :| FlowGraph.IsSimpleResidualPath(V, s, t, capacity, flow, pathToSource) && pathToSource[0] == u && pathToSource[|pathToSource|-1] == s;
 
-      height[u] := min_h + 1;
+      // Since u != s, the path has at least 2 nodes. Grab the next node in the path
+      assert |pathToSource| >= 2;
+      ghost var pathToSourceNextNode := pathToSource[1];
 
-      // Update the Highest-Label Buckets
-      // Add the node to its new, higher bucket (Stale Entry strategy: we don't remove the old one)
-      buckets[height[u]] := buckets[height[u]] + [u];
+      // Because u and path_v are connected on a residual path, there is residual capacity
+      assert FlowGraph.ResidualCapacity(V, s, t, capacity, flow, u, pathToSourceNextNode) > 0;
+
+      // get the remainder of the path (from path_v to s)
+      ghost var pathToSourceWithoutU := pathToSource[1..];
+
+      // Apply length and telescoping height lemmas
+      Graph.Lemma_SimplePathHasBoundedLength(V, pathToSource);
+      assert |pathToSource| <= V;
+      FlowGraph.Lemma_PathTelescopingHeight(V, s, t, capacity, flow, height, pathToSourceWithoutU);
+      assert height[pathToSourceNextNode] <= height[s] + |pathToSourceWithoutU| - 1;
+      // Since |pathToSource| <= V, the subpath has length <= V - 1
+      assert |pathToSourceWithoutU| <= V - 1;
+      // Since height[s] == V, we get:
+      assert height[pathToSourceNextNode] <= V + (V - 1) - 1;
+      assert height[pathToSourceNextNode] <= 2 * V - 2;
+      assert height[pathToSourceNextNode] < 2 * V - 1;
+
+      // This proves there exists a path to source where
+      // - height[pathToSourceNextNode] < 2 * V - 1
+      // minHeightNeighbourOfU is the neighbour on the path where the next node has the minimum height
+      // this means the following assertion also holds
+      assert minHeightNeighbourOfU < 2 * V - 1;
+
+      // Remove u from its old bucket
+      buckets[height[u]] := buckets[height[u]] - {u};
+
+      // Update u's height
+      height[u] := minHeightNeighbourOfU + 1;
+      // from these above lemmas we can thus conclude that height[u] falls within the bounds of the buckets
+      assert height[u] < 2 * V;
+
+      // Add u to its new, higher bucket
+      buckets[height[u]] := buckets[height[u]] + {u};
 
       // Because we lifted a node, it might be the new absolute highest active node
       if (height[u] > max_height) {
